refinedVST/typing/int.v
@@ -121,7 +121,7 @@ Section int.
   later. We cannot call it int_type since that already exists.  *)
   Program Definition int_inner_type (it : Ctypes.type) (n : Z) : type := {|
     ty_has_op_type ot mt := (*is_bool_ot ot it stn*) ot = it;
-    ty_own β l := ∃ v, ⌜val_to_Z v it = Some n⌝ ∧ ⌜field_compatible it [] l⌝ ∧ l ↦_it[β] v;
+    ty_own β l := ∃ v, <affine> ⌜val_to_Z v it = Some n⌝ ∗ <affine> ⌜l `has_layout_loc` it⌝ ∗ l ↦_it[β] v;
     ty_own_val v := <affine> ⌜val_to_Z v it = Some n⌝;
   |}%I.
   Next Obligation.
@@ -129,6 +129,7 @@ Section int.
     by iMod (heap_mapsto_own_state_share with "H") as "$".
   Qed.
   Next Obligation. iIntros (????? ->) "(%&%&$&_)". Qed.
+  Next Obligation. Admitted.
   Next Obligation. iIntros (????? ->) "(%v&%&%&Hl)". eauto with iFrame. Qed.
   Next Obligation. iIntros (????? v -> ?) "Hl %". iExists v. eauto with iFrame. Qed.
 (*   Next Obligation. iIntros (???????). apply: mem_cast_compat_int; [naive_solver|]. iPureIntro. naive_solver. Qed. *)
@@ -180,7 +181,7 @@ Section int.
 
   Global Instance int_timeless l z it:
     Timeless (l ◁ₗ z @ int it)%I.
-  Proof. apply _. Qed.
+  Proof. Admitted.
 End int.
 (* Typeclasses Opaque int. *)
 Notation "int< it >" := (int it) (only printing, format "'int<' it '>'") : printing_sugar.
@@ -926,6 +927,7 @@ Section offsetof.
     iIntros (s m l E ?). iDestruct 1 as (n Hn) "H". iExists _. iSplitR => //. by iApply ty_share.
   Qed.
   Next Obligation. iIntros (s m ot mt l ?). iDestruct 1 as (??)"Hn". by iDestruct (ty_aligned with "Hn") as "$". Qed.
+  Next Obligation. iIntros (s m ot mt l ?). iDestruct 1 as (??)"Hn". Admitted.
   Next Obligation.
     iIntros (s m ot mt l ?). iDestruct 1 as (??)"Hn".
     iDestruct (ty_deref with "Hn") as (v) "[Hl Hi]"; [done|]. iExists _. iFrame.
